src/Std/Data/DHashMap/Internal/WF.lean
@@ -51,6 +51,10 @@ theorem computeSize_eq {buckets : Array (AssocList α β)} :
 
 namespace Raw
 
+theorem equiv_iff_perm_toListModel [BEq α] [Hashable α] {m₁ m₂ : Raw α β} :
+    m₁ ≈ m₂ ↔ toListModel m₁.2 ~ toListModel m₂.2 :=
+  ⟨Raw.Equiv.perm_toListModel, Raw.Equiv.mk⟩
+
 theorem size_eq_length [BEq α] [Hashable α] {m : Raw α β} (h : Raw.WFImp m) :
     m.size = (toListModel m.buckets).length :=
   h.size_eq
